backends/lean/Base/Primitives/Scalar.lean
@@ -1301,12 +1301,24 @@ instance {ty} : LT (Scalar ty) where
 
 instance {ty} : LE (Scalar ty) where le a b := LE.le a.val b.val
 
--- Not marking this one with @[simp] on purpose
+-- Not marking this one with @[simp] on purpose: if we have `x = y` somewhere in the context,
+-- we may want to use it to substitute `y` with `x` somewhere.
+-- TODO: mark it as simp anyway?
 theorem Scalar.eq_equiv {ty : ScalarTy} (x y : Scalar ty) :
   x = y ↔ (↑x : Int) = ↑y := by
   cases x; cases y; simp_all
 
+-- Those theorems are safer to mark as `simp` however, I believe
+@[simp]
+theorem Scalar.eq_ofInt_right_equiv (x : Scalar ty) (y : Int) (h : Scalar.cMin ty ≤ y ∧ y ≤ Scalar.cMax ty) :
+  x = Scalar.ofInt y h ↔ x.val = y := by simp [Scalar.eq_equiv]
+
+@[simp]
+theorem Scalar.eq_ofInt_left_equiv (x : Scalar ty) (y : Int) (h : Scalar.cMin ty ≤ y ∧ y ≤ Scalar.cMax ty) :
+  Scalar.ofInt y h = x ↔ y = x.val := by simp [Scalar.eq_equiv]
+
 -- This is sometimes useful when rewriting the goal with the local assumptions
+-- TODO: this doesn't get triggered
 @[simp] theorem Scalar.eq_imp {ty : ScalarTy} (x y : Scalar ty) :
   (↑x : Int) = ↑y → x = y := (eq_equiv x y).mpr
 
